proof/infoflow/timeprotection/TimeProtectionIntegration.thy
@@ -2,7 +2,7 @@
  * Copyright 2021, UNSW (ABN 57 195 873 179),
  * Copyright 2021, The University of Melbourne (ABN 84 002 705 224).
  *
- * SPDX-License-Identifier: BSD-2-Clause
+ * SPDX-License-Identifier: GPL-2.0-only
  *)
 
 theory TimeProtectionIntegration
@@ -10,105 +10,94 @@ imports TimeProtection
   "InfoFlow.Noninterference"
 begin
 
-
-locale integration = 
-  Noninterference_valid_initial_state _ _ _ _ initial_aag +
-  tph?:time_protection_hardware
-    "TYPE('fch \<times> 'fch_cachedness \<times> 'pch \<times> 'pch_cachedness \<times> 'partition \<times> 'colour)"
-  (* re-fixed here just to align the 'partition type *)
-  for initial_aag :: "'partition subject_label PAS"
-begin
-
-type_alias tpdomain = TimeProtection.domain
-
 type_synonym if_other_state = "(user_context \<times> det_ext Structures_A.state) \<times> sys_mode"
 
-\<comment> \<open> since we define the 'domain' type in TimeProtection, we need to convert the
-    'partition' type from InfoFlow indo this type (and back)\<close>
-definition partition_to_domain :: "'partition partition \<Rightarrow> 'partition tpdomain" where
-  "partition_to_domain p \<equiv> case p of
-                             PSched \<Rightarrow> Sched |
-                             Partition x \<Rightarrow> User x"
+locale integration_setup = 
+  time_protection_hardware
+    gentypes
+    PSched +
+  Noninterference_valid_initial_state _ _ _ _ initial_aag
+  for gentypes :: "('fch \<times> 'fch_cachedness \<times> 'pch \<times> 'pch_cachedness \<times> 'l partition \<times> 'colour) itself"
+  and initial_aag :: "'l subject_label PAS"
++ fixes nlds :: "time \<Rightarrow> time"
+  fixes ta :: "if_other_state \<Rightarrow> vpaddr set"
+begin
 
-definition domain_to_partition :: "'partition tpdomain \<Rightarrow> 'partition partition" where
-  "domain_to_partition d \<equiv> case d of
-                             Sched \<Rightarrow> PSched |
-                             User x \<Rightarrow> Partition x"
+interpretation tphuwr:time_protection_hardware_uwr gentypes PSched 
+  _ _ _ _ _ _ _ _ _ _ _ _ _ _ _ _ _ _ part uwr nlds ta
+  apply unfold_locales
+   apply (simp add: schedIncludesCurrentDom)
+  using uwr_equiv_rel apply blast
+  done
 
-lemma partition_is_domain [simp]:
-  "domain_to_partition (partition_to_domain p) = p"
-  by (clarsimp simp:partition_to_domain_def domain_to_partition_def split:partition.split)
+abbreviation ma_uwr where "ma_uwr \<equiv> tphuwr.uwr"
 
-lemma domain_is_partition [simp]:
-  "partition_to_domain (domain_to_partition d) = d"
-  by (clarsimp simp:partition_to_domain_def domain_to_partition_def split:domain.split)
-
-\<comment> \<open> parameters to the tp locales \<close>
+(*
+(* the definition used in infoflow *)
 definition if_A where
   "if_A \<equiv> big_step_ADT_A_if utf"
 
 definition if_s0 where
   "if_s0 \<equiv> s0"
 
-definition if_current_domain :: "if_other_state \<Rightarrow> 'partition tpdomain" where
-  "if_current_domain os \<equiv> partition_to_domain (part os)"
+definition if_current_domain :: "if_other_state \<Rightarrow> 'l partition" where
+  "if_current_domain \<equiv> part"
 
-definition if_uwr :: "'partition tpdomain \<Rightarrow> (if_other_state \<times> if_other_state) set" where
-  "if_uwr d \<equiv> uwr (domain_to_partition d)"
+definition if_uwr :: "'l partition \<Rightarrow> (if_other_state \<times> if_other_state) set" where
+  "if_uwr d \<equiv> uwr d"
 
-(*FIXME: all of this domain/policy stuff is getting messy *)
-definition if_policy :: "('partition tpdomain \<times> 'partition tpdomain) set" where
-  "if_policy \<equiv> {(u, u'). policy2 (domain_to_partition u) (domain_to_partition u')}"
+(* the definition used in infoflow *)
+definition if_policy :: "('l partition \<times> 'l partition) set" where
+  "if_policy \<equiv> policyFlows (pasPolicy initial_aag)"
+ *)
 
-thm confidentiality_u
+end
 
+locale integration =
+  ii?:integration_setup _ _ _ _ _ _ _ _ _ _ _ _ _ _ _ _ _ _ _ _ _ _ _ _ _ _ _ gentypes +
+  ts?:trace_selector
+    "TYPE((if_other_state \<times> ('fch, 'pch) TimeProtection.state) \<times> 'l partition \<times> trace \<times> vpaddr set)"
+    "ii.part \<circ> fst" ma_uwr PSched "[]" "step_is_uwr_determined \<circ> fst" "step_is_publicly_determined \<circ> fst" select_trace 
+  for gentypes :: "('fch \<times> 'fch_cachedness \<times> 'pch \<times> 'pch_cachedness \<times> 'l partition \<times> 'colour) itself"
+  and select_trace and step_is_uwr_determined and step_is_publicly_determined
+begin
 
-interpretation ma?:time_protection_system _ if_A if_s0 if_current_domain if_uwr if_policy
-  apply unfold_locales
-
-
-  (*
-  fixes
-    select_trace ::
-      "('other_state \<times> ('fch, 'pch) state \<Rightarrow> (vaddr \<times> paddr) set \<Rightarrow> trace_unit list set)
-       \<Rightarrow> 'other_state \<times> ('fch, 'pch) state \<Rightarrow> (vaddr \<times> paddr) set \<Rightarrow> trace_unit list"
-    and A :: "('a, 'other_state, unit) data_type"
-    and s0 :: "'other_state"
-    and current_domain :: "'other_state \<Rightarrow> 'userdomain domain"
-    and external_uwr :: "'userdomain domain \<Rightarrow> ('other_state \<times> 'other_state) set"
-    and policy :: "('userdomain domain \<times> 'userdomain domain) set"
-    and out :: "'userdomain domain \<Rightarrow> 'other_state \<Rightarrow> 'p"
-    and collides_in_pch :: "paddr \<Rightarrow> paddr \<Rightarrow> bool"  (infix \<open>coll\<close> 50)
-    and fch_lookup :: "'fch \<Rightarrow> vaddr \<Rightarrow> 'fch_cachedness"
-    and pch_lookup :: "'pch \<Rightarrow> paddr \<Rightarrow> 'pch_cachedness"
-    and fch_read_impact :: "vaddr \<Rightarrow> 'fch \<Rightarrow> 'fch"
-    and pch_read_impact :: "paddr \<Rightarrow> 'pch \<Rightarrow> 'pch"
-    and fch_write_impact :: "vaddr \<Rightarrow> 'fch \<Rightarrow> 'fch"
+(*
+pch_read_impact :: "paddr \<Rightarrow> 'pch \<Rightarrow> 'pch"
     and pch_write_impact :: "paddr \<Rightarrow> 'pch \<Rightarrow> 'pch"
-    and read_cycles :: "'fch_cachedness \<Rightarrow> 'pch_cachedness \<Rightarrow> nat"
-    and write_cycles :: "'fch_cachedness \<Rightarrow> 'pch_cachedness \<Rightarrow> nat"
-    and empty_fch :: "'fch"
-    and fch_flush_cycles :: "'fch \<Rightarrow> nat"
-    and pch_flush_WCET :: "paddr set \<Rightarrow> nat"
-    and fch_flush_WCET :: "nat"
     and do_pch_flush :: "'pch \<Rightarrow> paddr set \<Rightarrow> 'pch"
     and pch_flush_cycles :: "'pch \<Rightarrow> paddr set \<Rightarrow> nat"
-    and addr_domain :: "paddr \<Rightarrow> 'userdomain domain"
+    and pch_flush_WCET :: "paddr set \<Rightarrow> nat"
+    and collides_in_pch :: "paddr \<Rightarrow> paddr \<Rightarrow> bool"  (infix \<open>coll\<close> 50)
+    and read_cycles :: "'fch_cachedness \<Rightarrow> 'pch_cachedness \<Rightarrow> nat"
+    and write_cycles :: "'fch_cachedness \<Rightarrow> 'pch_cachedness \<Rightarrow> nat"
+    and addr_domain :: "paddr \<Rightarrow> 'domain"
     and addr_colour :: "paddr \<Rightarrow> 'colour"
-    and colour_userdomain :: "'colour \<Rightarrow> 'userdomain"
-    and touched_addrs :: "'other_state \<Rightarrow> (vaddr \<times> paddr) set"
-    and step_is_publicly_determined :: "'other_state \<Rightarrow> bool"
-    and step_is_uwr_determined :: "'other_state \<Rightarrow> bool"
-    and next_latest_domainswitch_start :: "nat \<Rightarrow> nat"
-    and will_domain_switch :: "'other_state \<Rightarrow> bool"
-    and domainswitch_start_delay_WCT :: "nat"
-    and dirty_step_WCET :: "nat"
-    and initial_pch :: "'pch"
-    and get_next_domain :: "'other_state \<Rightarrow> 'userdomain domain"
-    and get_domainswitch_middle_state :: "'other_state \<Rightarrow> 'other_state"
-    and get_domainswitch_final_state :: "'other_state \<Rightarrow> 'other_state"
-    and step_is_only_timeprotection_gadget :: "'other_state \<Rightarrow> 'other_state \<Rightarrow> bool"
-*)
+    and colour_userdomain :: "'colour \<Rightarrow> 'domain"
+ *)
+
+interpretation ma?:time_protection_system PSched fch_lookup fch_read_impact fch_write_impact
+  empty_fch fch_flush_cycles fch_flush_WCET pch_lookup pch_read_impact pch_write_impact do_pch_flush
+  pch_flush_cycles pch_flush_WCET collides_in_pch read_cycles write_cycles addr_domain addr_colour colour_userdomain
+  part uwr nlds ta select_trace
+  "big_step_ADT_A_if utf" s0 "policyFlows (pasPolicy initial_aag)" _
+  
+  apply unfold_locales
+               using schedIncludesCurrentDom apply presburger
+              apply (simp add: uwr_equiv_rel)
+             subgoal sorry
+            subgoal sorry
+           subgoal sorry
+          subgoal sorry
+         subgoal sorry
+        subgoal sorry
+       subgoal sorry
+      subgoal sorry
+     subgoal sorry
+    subgoal sorry
+   subgoal sorry
+  subgoal sorry
+  done
 end
 
 end
